\section{Hoare Logic}

\newcommand{\true}{\textsf{true}}
\newcommand{\len}[1]{\textsf{len}(#1)}
\newcommand{\dom}{{\sf dom}}
\newcommand{\ifstmt}[3]{{\sf if}~#1~{\sf then}~#2~{\sf else}~#3}
\newcommand{\whilestmt}[2]{{\sf while}~#1~{\sf do}~#2}
\newcommand{\X}{\textsf{X}}

\begin{enumerate}[(a)]
% TODO: consider adding dom_a(X) checks
\item \begin{eqnarray*}
    \dom_a(\bar{n})        & = & {\sf true} \\
    \dom_a(x)              & = & {\sf true} \\
    \dom_a(a_0 \oplus a_1) & = & \dom_a(a_0) \wedge \dom_a(a_1) \\
    \dom_a({\sf X}[a])     & = & 0 \leq a \wedge a < {\sf len(X)} \\
    \dom_a({\sf len(X)})   & = & {\sf true} \\
\end{eqnarray*}

\begin{eqnarray*}
    \dom_b({\sf true})      & = & {\sf true} \\
    \dom_b({\sf false})     & = & {\sf true} \\
    \dom_b(a_0 \odot a_1)   & = & \dom_a(a_0) \wedge \dom_a(a_1) \\
    \dom_b(b_0 \oslash b_1) & = & \dom_b(b_0) \wedge \dom_b(b_1) \\
    \dom_b(\neg b)          & = & \dom_b(b) \\
\end{eqnarray*}

\item
$
\Rule{SimpleAssign}{}{
    \{ \dom_a(a) \wedge P[a / x]\}
    x := a
    \{ P \}
}
$
\\

$
\Rule{ArrayAssign}{}{
    \{ \dom_a({\sf X}[a_0]) \wedge \dom_a(a_1) \wedge P[{\sf X}[a_0 \mapsto a_1] / X \}
    {\sf X}[a_0] := a_1
    \{ P \}
}
$
\\

$
\Rule{If}{
    \{ b \wedge P \}
    c_1
    \{ Q \}
    \\
    \{ \neg b \wedge P \}
    c_2
    \{ Q \}
}{
    \{ \dom_b(b) \wedge P \}
    \ifstmt{b}{c_1}{c_2}
    \{ Q \}
}
$
\\

$\Rule{While}{
    \{ b \wedge P \}
    c
    \{ P \}
}{
    \{ P \}
    \whilestmt{b}{c}
    \{ \neg b \wedge P \}
}$

\item
\begin{enumerate}[i.]
    \item
    \begin{eqnarray*}
        A_0 = & \forall k . & 0 \leq k < j - 1 \Rightarrow  {\sf X}[k] > {\sf X}[k + 1] \\
              & & \\
        A_1 = & \forall k. & (0 \leq k < j - 1) \Rightarrow \X[k] \geq \X[k + 1] \\
              & \wedge     & i < \len{\X} \\
    \end{eqnarray*}

    \item
    \begin{proof} \hspace{1cm} \\
        \begin{itemize}
        \item $\neg (j < {\sf len(X)})$ implies $j \geq {\sf len}(x)$
        \item we can apply $A_0$ to each $k$ in the range
        $[0, {\sf len}(x) - 2]$ to show that $P$ holds.
        \end{itemize}
    \end{proof}

    \item
    \begin{proof} We'll present the proof tree in three parts: Left-Tree will
        give a derivation for the first command, Right-Tree will give a
        derivation for the second, and an overall derivation will
        show how the proof trees can be combined. We'll present these trees
        in reverse order to reflect the way they were derived.

        \newcommand{\leftPremise}{
            \{ \dom_a(i + 1) \wedge \dom_a({\sf X}[i])
               \wedge A_1[i - 1 / i][i + 1 \mapsto \X[\X[i]
             \}
             ~\X[i = 1] = \X[i]~
             \{ A_1[i - 1/ i] \}
        }

        \newcommand{\leftBase}{
            \{ A_1 \wedge ((i \geq 0) \wedge {\sf X}[i] < x) \}
            ~\X[i = 1] = \X[i]~
            \{ A_1[i - 1/ i] \}
        }

        \newcommand{\rightPremise}{
            \{ \dom_a(i - 1) \wedge A_1[i - 1/ i] \}
            ~i = i - 1~
            \{ A_1 \}
        }

        \newcommand{\rightBase}{
            \{ A_1[i - 1/ i] \}
            ~i = i - 1~
            \{ A_1 \}
        }
        \newcommand{\treeBase}{
            \{ A_1 \wedge ((i \geq 0) \wedge {\sf X}[i] < x) \}
            ~\X[i + 1] = \X[i];~i = i - 1~
            \{ A_1 \}
        }

        \underline{Overall derivation}:

        $$ \inferrule{
                \text{Left-Tree}
                \\
                \text{Right-Tree}
            }{\treeBase}
        $$

        \underline{Right-Tree}: \\
        $$ \inferrule{\rightPremise}{\rightBase} $$

        Note that $\dom_a(i - 1)$ is always true by definition.

        \underline{Left-Tree}:  \\
        $$ \inferrule{\leftPremise}{\leftBase} $$

        This tree is difficult to read, so let's break it into simpler parts.
        The left-most proposition in the premise is the result of applying
        our rule for array assignments. It consists of 3 parts:

        \begin{itemize}
        \item $\dom_a(i + 1)$
        \item $\dom_a({\sf X}[i])$
        \item $A_1[i - 1 / i][\X[i + 1 \mapsto \X[i]]$
        \end{itemize}

        The last clause is equivalent to

        $$ i - 1 < {\sf len(X)} \wedge \forall k. (0 \leq k < j - 1) \Rightarrow \X[k] \geq \X[k + 1]$$

        These three clauses follow from $ A_1 \wedge ((i \geq 0) \wedge {\sf X}[i] < x) $

        \begin{itemize}
        \item $\dom_a(i + 1) = \dom_a(i) \wedge \dom_a(1) = \true $
        \item $\dom_a({\sf X}[i]) = 0 \leq i \wedge i < \len{\X} $ follows from
        $i \geq 0$ and $i < \len{\X}$ (the latter comes from $A_1$).
        \item This clause is just a weakened version of $A_1$. Note that the right
        clause of the conjunction is the same and that
        $i < \len{\X} \Rightarrow i - 1 < \len{\X}$, the left clause of the
        conjunction.

        % $A_1$ satisfies leads directly to most parts of the third clause. What's unclear is whether the $forall k$ proposition holds in the $k = i$ case.

        \end{itemize}




    \end{proof}
    \end{enumerate}


\end{enumerate}
