\section{Denesting Loops}

We first encode the code before and after the transformation into a KAT of elements from $K$ and tests from $B \subseteq K$.
\begin{align*}
\texttt{while c do q} &= (cq)^*\overline c\\
\texttt{p; while c do q} &= p(cq)^*\overline c\\
\texttt{while b do \{p; while c do q\}} &= (bp(cq)^*\overline c)^*\overline b\\\\
\texttt{if c then q else p} &= cq + \overline c p\\
\texttt{while b $\vee$ c do \{if c then q else p\}} &= ((b + c)(cq + \overline c p))^*\overline{(b+c)}\\
\texttt{if b then \{p; while b $\vee$ c do \{if c then q else p\}\}} &= bp((b + c)(cq + \overline c p))^*\overline{(b+c)}+ \overline b 1
\end{align*}

We wish to prove that $(bp(cq)^*\overline c)^*\overline b = (bp((b + c)(cq + \overline c p))^*\overline{(b+c)})^*\overline b + \overline b 1$.

First note that $b, c$ and $1$ are elements of the Boolean algebra in $B$. We can treat $b$ and $c$ as truth variables, $1$ as T (true), $+$ as $\vee$ and $.$ as $\wedge$. With this we can claim the following identities before proving the equality above.
\begin{align*}
\overline{(b+c)} &= \overline {cb} \text{ (by De Morgan's law)}\\
\overline b 1 &= \overline b\\
(b + c)(cq + \overline c p) &= bcq + b \overline c p + ccq + c \overline c p\\
&= bcq + b \overline c p + cq \text{ (since $cc = c$ and $c \overline c = 0$)}\\
&= bcq + cq + b \overline c p \text{ (since $+$ is commutative)}\\
&= (b+1)cq + b \overline c p \text{ (by distributivity)}\\
&= cq + b \overline c p \text{ (since $b + 1 = 1$)}\\
&= cq + \overline c b p \text{ (by commutativity of $.$ in $B$)}\\
\Rightarrow ((b + c)(cq + \overline c p))^* &= (cq + \overline c b p)^*\\
&= ((cq)^*\overline c b p)^* (cq)^* \text{ (since $(p+q)^* = (p^*q)^*p^*$}\\
\Rightarrow RHS &= bp((b + c)(cq + \overline c p))^*\overline{(b+c)}+ \overline b 1\\
&= bp((b + c)(cq + \overline c p))^*\overline{cb}+ \overline b\\
&= (bp((b + c)(cq + \overline c p))^*\overline c + 1)\overline b\\
&= (bp((cq)^*\overline c b p)^* (cq)^*\overline c + 1)\overline b\\
&= (bp(cq)^*\overline c (b p (cq)^*)\overline c)^* + 1)\overline b \text{ (since $(pq)^*p = p(qp)^*$)}\\
&= (bp(cq)^*\overline c)^*\overline b \text{ (since $pp^* +1 = p^*$)}\\
&= LHS~\Box
\end{align*}