\section{Encoding Sums as Products}
\begin{enumerate}[(a)]
  \item
  Recall that the type $\forall\alpha.\alpha$ is uninhabited so we can use this as the type void that represents False.

  We claim that $\phi \vee \psi \equiv \forall \alpha.(((\phi \rightarrow \alpha) \times (\psi \rightarrow \alpha)) \rightarrow \alpha)$.

  $((\phi \rightarrow \alpha) \times (\psi \rightarrow \alpha)) \rightarrow \alpha$ is true if and only if either $\phi, \psi$ or $\alpha$ is true. Since this has to hold for all $\alpha$, the proposition $\forall \alpha.(((\phi \rightarrow \alpha) \times (\psi \rightarrow \alpha)) \rightarrow \alpha)$ is true if and only if either $\phi$ or $\psi$ is true. 

  % \begin{align*}
  % \phi \vee \psi &\equiv \neg (\neg \phi \wedge \neg \psi)\\
  %                &\equiv ((\phi \rightarrow \perp) \times (\psi \rightarrow \perp)) \rightarrow \perp\\
  %                &\equiv ((\phi \rightarrow \forall \alpha.\alpha) \times (\psi \rightarrow \forall ~\alpha.\alpha)) \rightarrow \forall \alpha.\alpha\\
  % \end{align*}
  %%%%%%%%%%%%%%%%%%%%%%%%%%%%%%%%%%%%%%%%%%%%%%%%%%%%
   \item
   \begin{align*}
    \T {\texttt{unit}} &\triangleq \texttt{unit}\\
    \T {\tau_1 \rightarrow \tau_2} &\triangleq \T {\tau_1} \rightarrow \T {\tau_2}\\
    \T {\tau_1 + \tau_2} &\triangleq \forall\alpha.((\T {\tau_1} \rightarrow \alpha) \times (\T {\tau_2} \rightarrow \alpha)) \rightarrow \alpha
   \end{align*}
   \item
   \begin{align*}
    \E {\texttt{inL}_{\tau_1 + \tau_2}e} &\triangleq \Lambda \alpha.\lambda f : ((\T {\tau_1} \rightarrow \alpha) \times (\T {\tau_2} \rightarrow \alpha)). ((\#1~f)~\E{e})\\
    \E {\texttt{inR}_{\tau_1 + \tau_2}e} &\triangleq \Lambda \alpha.\lambda f : ((\T {\tau_1} \rightarrow \alpha) \times (\T {\tau_2} \rightarrow \alpha)). ((\#2~f)~\E{e})\\
    \E {\texttt{case $e_0$ of $e_1$|$e_2$}} &\triangleq \E {e_0}~\T {\beta}~(\E{e_1}, \E{e_2}) \\
    &\texttt{where $e_1$ and $e_2$ both map into type $\beta$}
   \end{align*}
\end{enumerate}